theories/LambdaWP.v
@@ -275,8 +275,8 @@ Definition wp_for_val (v1 v2:val) (F1:val->formula) : formula := local (fun Q =>
 
 Definition wp_case (v:val) (p:pat) (F1:ctx->formula) (F2:formula) : formula :=
   local (fun Q => 
-    hand (\forall (G:ctx), \[v = patsubst G p] \-* F1 G Q)
-         (\[forall (G:ctx), v <> patsubst G p] \-* F2 Q) ).
+    hand (\forall (G:ctx), \[Ctx.dom G = patvars p /\ v = patsubst G p] \-* F1 G Q)
+         (\[forall (G:ctx), Ctx.dom G = patvars p -> v <> patsubst G p] \-* F2 Q) ).
 
 
 (* ---------------------------------------------------------------------- *)
@@ -310,8 +310,7 @@ Fixpoint wp (E:ctx) (t:trm) : formula :=
       end
   | trm_case t1 p t2 t3 => 
      match t1 with
-     | trm_val v1 => wp_case v1 p (fun (G:ctx) => wp (Ctx.app (Ctx.rem_vars (patvars p) E) G) t2) (aux t3)
-                  (* TODO wp (Ctx.app G E) t2 *)
+     | trm_val v1 => wp_case v1 p (fun (G:ctx) => wp (Ctx.app G E) t2) (aux t3)
      | _ => wp_fail
      end
   | trm_fail => wp_fail
@@ -545,40 +544,17 @@ Proof using. Opaque Ctx.add Ctx.rem.
   { rewrite~ triple_eq_himpl_wp_triple. }
 Qed.
 
-Lemma isubst_app_eq_isubst_isubst : forall G E t,
-  isubst (Ctx.app G E) t = isubst E (isubst G t).
-Proof using.
-  intros G. induction G as [|(y,w) G']; intros; simpl.
-  { rewrite~ isubst_nil. }
-  { do 2 rewrite isubst_cons. rewrite~ IHG'. }
-Qed.
-
-Lemma isubst_app_eq_isubst_isubst_rem_vars : forall G E t p,
-  isubst (Ctx.app G E) t = isubst G (isubst (Ctx.rem_vars (patvars p) E) t).
-Proof using.
-  intros G. induction G as [|(y,w) G']; intros.
-  { simpl. rewrite isubst_nil. 
-skip. } skip.
-Qed.
-
-Lemma isubst_eq : forall G E p t,
-  isubst (Ctx.app (Ctx.rem_vars (patvars p) E) G) t = isubst (Ctx.app G E) t.
-Proof using.
-  skip.
-Qed.
-
-
-Lemma wp_sound_case : forall v1 p F1 F2 t1 t2 E, (* TODO (wp_triple_ G E t1) *)
-  (forall (G:ctx), F1 G ===> wp_triple_ (Ctx.app (Ctx.rem_vars (patvars p) E) G) t1) ->
+Lemma wp_sound_case : forall v1 p F1 F2 t1 t2 E,
+  (forall (G:ctx), F1 G ===> wp_triple_ (Ctx.app G E) t1) ->
   F2 ===> wp_triple_ E t2 ->
   wp_case v1 p F1 F2 ===> wp_triple_ E (trm_case v1 p t1 t2).
 Proof using.
   introv M1 M2. applys qimpl_wp_triple. simpl. intros Q.
   remove_local. applys triple_case.
-  { intros G Hv1. applys triple_hand_l. applys triple_hforall_for G.
+  { intros G HG Hv1. rewrites <- (rm HG).
+    applys triple_hand_l. applys triple_hforall_for G.
     applys~ triple_hwand_hpure_l. rewrite triple_eq_himpl_wp_triple.
-    rewrite <- isubst_app_eq_isubst_isubst.
-    (* TODO rewrite <- isubst_app_eq_isubst_isubst_rem_vars. *) applys M1. }
+    rewrite <- isubst_app_eq_isubst_isubst_rem_vars. applys M1. }
   { introv Hv1. applys triple_hand_r. applys* triple_hwand_hpure_l. 
     rewrite triple_eq_himpl_wp_triple. applys M2. }
 Qed.
